Racket/monad.rkt
@@ -1,0 +1,95 @@
+#lang plai-typed
+
+(define-type (Maybe 'a)
+  (Just (v : 'a))
+  (Error))
+
+
+; bad stype
+(define devide : ((Maybe number) (Maybe number) -> (Maybe number))
+  (lambda (x y)
+    (type-case (Maybe number) x
+      (Just (vx)
+            (type-case (Maybe number) y
+              (Just (vy) (if (= vy 0) (Error) (Just (/ vx vy))))
+              (Error () (Error))))
+      (Error () (Error)))))
+
+
+
+;try another way
+(define tedious-stuff : ((Maybe number) (number -> (Maybe number)) -> (Maybe number))
+  (lambda (k f)
+    (type-case (Maybe number) k
+      (Just (vk) (f vk))
+      (Error () (Error)))))
+
+
+(define devide2 : ((Maybe number) (Maybe number) -> (Maybe number))
+  (lambda (x y)
+    (tedious-stuff x
+                   (lambda (vx)
+                     (tedious-stuff y
+                                    (lambda (vy)
+                                      (if (= 0 vy)
+                                          (Error)
+                                          (Just (/ vx vy)))))))))
+
+;define a syntex
+(define-syntax do
+  (syntax-rules (<-)
+                [(do (vx <- x) (vy <- y) e)
+                 (tedious-stuff x
+                    (lambda (vx)
+                      (tedious-stuff y
+                         (lambda (vy)
+                           e))))]))
+;final version
+(define devide3 : ((Maybe number) (Maybe number) -> (Maybe number))
+  (lambda (x y)
+    (do (a <- x)
+        (b <- y)
+        (if (= b 0) (Error) (Just (/ a b))))))
+
+
+;other function
+(define my-add ; ((Maybe number) (Maybe number) -> (Maybe number))
+  (lambda (x y)
+    (do (a <- x)
+        (b <- y)
+        (Just (+ a b)))))
+
+
+;Do we need to redefine all functions? of course not!
+;we can 'lift' functions to work as intended
+(define lift ; (('a 'b -> 'c) (Maybe 'a) (Maybe 'b) -> (Maybe 'c))
+  (lambda (f)
+    (lambda (x y)
+      (do (a <- x)
+          (b <- y)
+          (Just (f a b))))))
+
+(define my-add2 (lift +))
+
+;;;
+;A monad is completely defined by:
+;• A type constructor to have values of type M A
+;• A ’unit’ or ’return’ function with type A -> M A
+;• A ’bind’ function with type: M A -> (A -> MB) -> M B
+
+
+;Maybe Monad
+
+;Type constructor :
+;(define-type Maybe (Just (v any?)) (Error))
+
+;Unit:
+; A -> Maybe A
+;(define (unit v) (Just v))
+
+;Binder:
+; M A -> (A -> M B) -> M B
+;(define (bind k f)
+;    (type-case Maybe k
+;      (Just (v) (f v))
+;      (Error () (Error))))
