Coq/Software Foundation/R_hoare2.v
@@ -1,0 +1,143 @@
+(*
+  contents:
+  1. Decorated Programs
+  2.
+  3.
+  4.
+  5.
+*)
+
+Require Import Coq.Bool.Bool.
+Require Import Coq.Arith.Arith.
+Require Import Coq.Arith.EqNat.
+Require Import Coq.omega.Omega.
+Require Import H_maps.
+Require Import L_imp.
+Require Import Q_hoare.
+
+
+
+
+
+(* Decorated Programs *)
+(*------------------------------------------------------------*)
+(*
+The beauty of Hoare Logic is that it is compositional: the 
+structure of proofs exactly follows the structure of programs.
+
+a decorated program consists of the program text interleaved with 
+assertions (either a single assertion or possibly two assertions 
+separated by an implication). To check that a decorated program 
+represents a valid proof, we check that each individual command is 
+locally consistent with its nearby assertions
+*)
+
+Definition reduce_to_zero' : com :=
+  WHILE BNot (BEq (AId X) (ANum 0)) DO
+    X ::= AMinus (AId X) (ANum 1)
+  END.
+
+Theorem reduce_to_zero_correct' :
+  {{fun st => True}}
+  reduce_to_zero'
+  {{fun st => st X = 0}}.
+Proof.
+  unfold reduce_to_zero'.
+  eapply hoare_consequence_post.
+  -apply hoare_while.
+   eapply hoare_consequence_pre.
+   +apply hoare_asgn.
+   +unfold assert_implies, bassn, assn_sub. simpl.
+    intros. reflexivity.
+  -unfold assert_implies, bassn, assn_sub. simpl.
+   intros. inversion H. destruct (st X =? 0) eqn:Hx.
+   apply beq_nat_true in Hx. assumption. simpl in H1.
+   destruct H1. auto.
+Qed.
+
+
+
+
+
+
+(*Finding Loop Invariants*)
+(*------------------------------------------------------------*)
+(*
+Once the outermost precondition and postcondition are chosen, 
+the only creative part in verifying programs using Hoare Logic is 
+finding the right loop invariants.
+
+it must be weak enough to be implied by the loop's precondition
+it must be strong enough to imply the program's postcondition
+it must be preserved by one iteration of the loop
+
+One way to find an invariant that satisfies these three 
+conditions is by using an iterative process: start with a 
+"candidate" invariant (a guess or a heuristic choice) and check 
+the three conditions above; if any of the checks fails, try to 
+use the information that we get from the failure to produce 
+another candidate invariant, and repeat the process.
+
+Very often, even if a variable is used in a loop in a read-only 
+fashion, it is necessary to add to the loop invariant.
+*)
+
+(* exercise *)
+Fixpoint parity x :=
+  match x with
+  | 0 => 0
+  | 1 => 1
+  | S (S x') => parity x'
+  end.
+
+Lemma parity_ge_2 : forall x,
+  2 <= x ->
+  parity (x - 2) = parity x.
+Proof.
+  induction x; intro. reflexivity.
+  destruct x. inversion H. inversion H1.
+  simpl. rewrite <- minus_n_O. reflexivity.
+Qed.
+
+Lemma parity_lt_2 : forall x,
+  not (2 <= x) ->
+  parity (x) = x.
+Proof.
+  intros. induction x. reflexivity. destruct x. reflexivity. 
+  simpl. exfalso. apply H. omega.
+Qed.
+
+Theorem parity_correct : forall m,
+    {{ fun st => st X = m }}
+  WHILE BLe (ANum 2) (AId X) DO
+    X ::= AMinus (AId X) (ANum 2)
+  END
+    {{ fun st => st X = parity m }}.
+Proof.
+  intros m.
+  apply hoare_consequence_pre with 
+    (P' := (fun st => parity m = parity (st X))).
+  -eapply hoare_consequence_post.
+   +apply hoare_while.
+    eapply hoare_consequence_pre.
+    *apply hoare_asgn.
+    *unfold assert_implies, bassn, assn_sub. simpl.
+     intros. destruct H. rewrite H. unfold t_update. simpl.
+     destruct (st X) eqn:He.
+     ++inversion H0.
+     ++destruct n. ** inversion H0. **simpl. 
+       rewrite <- minus_n_O. auto.
+   +unfold assert_implies, bassn, assn_sub. simpl. intros.
+    destruct H. rewrite H. destruct (st X) eqn:Hx.
+    *simpl. reflexivity.
+    *destruct n. ++auto. ++destruct H0. reflexivity.
+  -unfold assert_implies, bassn, assn_sub. simpl. intros.
+   rewrite H. reflexivity.
+Qed.
+
+
+
+
+
+
+(*------------------------------------------------------------*)
